some progress on the Minify proof.

theories/RTac/Minify.v
@@ -13,6 +13,7 @@ Require Import MirrorCore.RTac.Reduce.
 Require Import MirrorCore.Util.Forwardy.
 Require Import MirrorCore.Util.Nat.
 
+
 Set Implicit Arguments.
 Set Strict Implicit.
 
@@ -32,14 +33,14 @@ Section parameterized.
     (** [es] must be pre-translated **)
 
     Fixpoint lookup_compress (es : list (option expr)) (base u : uvar)
-    : option expr :=
+    : expr :=
       match es with
-        | nil => Some (UVar (base + u)) (* DEAD *)
+        | nil => (UVar (base + u)) (* DEAD *)
         | e :: es' =>
           match e , u with
-            | None , 0 => Some (UVar base)
+            | None , 0 => (UVar base)
             | None , S u => lookup_compress es' (S base) u
-            | Some e' , 0 => Some e'
+            | Some e' , 0 => e'
             | Some _ , S u => lookup_compress es' base u
           end
       end.
@@ -51,19 +52,19 @@ Section parameterized.
     match lt_rem u base with
       | None => (* u < base *)
         ctx_lookup u cs
-      | Some u' => lookup_compress es base u'
+      | Some u' => Some (lookup_compress es base u')
     end.
 
   Section minify.
     Variable base : nat.
-    Variables (c : Ctx typ expr)
-              (cs : ctx_subst c).
+    Variables (c : Ctx typ expr) (cs : ctx_subst c).
+
     Fixpoint minify_goal (es : list (option expr))
              (nus : nat)  (g : Goal typ expr)
     : Goal typ expr :=
       match g with
         | GAll t g' =>
-          GAll t (minify_goal es nus g')
+          GAll_do_solved t (minify_goal es nus g')
         | GExs ts m g' =>
           let len_ts := length ts in
           let mlist := amap_aslist m nus len_ts in
@@ -76,49 +77,703 @@ Section parameterized.
                                          | None => true
                                          | Some _ => false
                                        end) tes in
-          let (ts',_) := split tes' in
+          let ts' := map fst tes' in
           GExs_nil_check ts' (amap_empty _)
                          (minify_goal (es ++ mlist_inst) (len_ts + nus) g')
         | GHyp e g' =>
-          GHyp (instantiate (do_instantiate cs base es) 0 e)
-               (minify_goal es nus g')
+          GHyp_do_solved (instantiate (do_instantiate cs base es) 0 e)
+                         (minify_goal es nus g')
         | GConj_ g1 g2 =>
-          GConj (minify_goal es nus g1)
-                (minify_goal es nus g2)
+          GConj (minify_goal es nus g1) (minify_goal es nus g2)
         | GGoal e =>
           GGoal (instantiate (do_instantiate cs base es) 0 e)
         | GSolved => GSolved
       end.
 
-    Lemma WellFormed_Goal_GConj : forall tus tvs a b,
-                                    WellFormed_Goal (typ:=typ) tus tvs a ->
-                                    WellFormed_Goal tus tvs b ->
-                                    WellFormed_Goal tus tvs (GConj a b).
+    Hypothesis base_is_nus : base = length (getUVars c).
+
+    (** TODO: These are all probably redundant **)
+    Lemma WellFormed_Goal_GConj
+      : forall tus tvs a b,
+        WellFormed_Goal (typ:=typ) tus tvs a ->
+        WellFormed_Goal tus tvs b ->
+        WellFormed_Goal tus tvs (GConj a b).
     Proof.
       destruct a; destruct b; simpl; intros; auto; constructor; auto.
     Qed.
 
-    Lemma minify_goal_sound
-    : forall g tus tvs,
-        WellFormed_Goal (getUVars c ++ tus) (getVars c ++ tvs) g ->
-        forall es,
-        WellFormed_Goal (getUVars c ++ tus) (getVars c ++ tvs)
-                        (minify_goal es (length (getUVars c ++ tus)) g).
+    Lemma WellFormed_Goal_GAll_do_solved
+      : forall tus tvs t g,
+        WellFormed_Goal tus tvs (GAll t g) ->
+        WellFormed_Goal tus tvs (GAll_do_solved t g).
     Proof.
-      induction 1; simpl; try solve [ constructor; eauto ].
-      { intros.
-        match goal with
-          | |- WellFormed_Goal _ _ match ?X with _ => _ end =>
-            consider X; intros
-        end.
-        destruct l. simpl.
-        rewrite Plus.plus_comm.
-        rewrite <- app_length.
-        admit. admit. }
-      { intros.
-        eapply WellFormed_Goal_GConj; auto. }
+      intros. destruct g; try eassumption.
+      do 2 constructor.
     Qed.
 
+    Lemma WellFormed_Goal_GHyp_do_solved
+      : forall tus tvs t g,
+        WellFormed_Goal tus tvs (GHyp t g) ->
+        WellFormed_Goal tus tvs (GHyp_do_solved t g).
+    Proof.
+      intros. destruct g; try eassumption.
+      do 2 constructor.
+    Qed.
+
+    (** TODO: I can not capture the meaning of the terms in the list without
+     ** their corresponding environments
+     **)
+
+    Inductive mapD (_tus _tus' _tvs : tenv typ)
+    : forall tus tus' (es : list (option expr)),
+        (hlist typD _tus -> hlist typD _tus' -> hlist typD _tvs ->
+         hlist typD tus -> hlist typD tus' -> Prop) -> Prop :=
+    | MD_nil : forall tus, @mapD _tus _tus' _tvs tus tus nil (fun _ _ _ a b => a = b)
+    | MD_None : forall es t tus tus' P,
+        @mapD (_tus ++ t :: nil) (_tus' ++ t :: nil) _tvs tus tus' es P ->
+        @mapD _tus _tus' _tvs (t :: tus) (t :: tus') (None :: es)
+              (fun U U' V a b =>
+                    hlist_hd a = hlist_hd b
+                 /\ P (hlist_app U (Hcons (hlist_hd a) Hnil))
+                      (hlist_app U' (Hcons (hlist_hd a) Hnil)) V
+                      (hlist_tl a) (hlist_tl b))
+    | MD_Some : forall e es t tus tus' P eD,
+        @mapD (_tus ++ t :: nil) _tus' _tvs tus tus' es P ->
+        exprD' (_tus' ++ tus') _tvs e t = Some eD ->
+        @mapD _tus _tus' _tvs (t :: tus) tus' (Some e :: es)
+              (fun U U' V a b =>
+                    hlist_hd a = eD (hlist_app U' b) V
+                 /\ P (hlist_app U (Hcons (hlist_hd a) Hnil))
+                      U' V (hlist_tl a) b).
+
+    Arguments mapD {_ _ _} _ _ _ _.
+
+    (** TODO(gmalecha): move **)
+    Lemma nth_error_get_hlist_nth_conv
+      : forall T F ls ls' n (pf : ls' = ls),
+        @nth_error_get_hlist_nth T F ls n =
+        match pf in _ = ls'
+              return option { t : T & hlist F ls' -> F t }
+        with
+          | eq_refl => @nth_error_get_hlist_nth T F ls' n
+        end.
+    Proof.
+      destruct pf; reflexivity.
+    Qed.
+    (** TODO(gmalecha): move to ExtLib.Data.SigT **)
+    Lemma eq_sigT_rw
+      : forall T U F (a b : T) (pf : a = b) s,
+        match pf in _ = x return @sigT U (F x) with
+          | eq_refl => s
+        end =
+        @existT U (F b) (projT1 s)
+                match pf in _ = x return F x (projT1 s) with
+                  | eq_refl => (projT2 s)
+                end.
+    Proof. destruct pf. destruct s; reflexivity. Qed.
+
+    Hint Rewrite eq_sigT_rw : eq_rw.
+
+    Lemma exprD'_UVar_ok
+      : forall tus tvs u t get,
+        nth_error_get_hlist_nth typD tus u = Some (@existT _ _ t get) ->
+        exists eD,
+          exprD' tus tvs (UVar u) t = Some eD /\
+          forall us vs, get us = eD us vs.
+    Proof.
+      intros.
+      generalize (@UVar_exprD' typ expr _ _ _ _ tus tvs u t).
+      destruct (exprD' tus tvs (UVar u) t).
+      { intros; forward_reason.
+        rewrite H in H0. inv_all. subst. eauto. }
+      { eapply nth_error_get_hlist_nth_Some in H. simpl in H.
+        forward_reason. destruct 1; try congruence.
+        exfalso. clear H. rewrite x in H0.
+        forward_reason. inv_all. apply H0. assumption. }
+    Qed.
+
+    (** NOTE: This proof is ugly b/c of all of the extraction operations
+     **)
+    Lemma lookup_compress_sound
+    : forall (_tus _tus' tus tus' tvs : list typ)
+             (es : list (option expr))
+             (R : hlist typD _tus -> hlist typD _tus' ->
+                  hlist typD tvs -> hlist typD tus -> hlist typD tus' -> Prop),
+        mapD tus tus' es R ->
+        forall (u : nat) (t : typ)
+               (get : hlist typD (_tus ++ tus) -> typD t),
+          nth_error_get_hlist_nth typD (_tus ++ tus) u =
+          Some (existT (fun t0 : typ => hlist typD (_tus ++ tus) -> typD t0) t get) ->
+          length _tus >= length _tus' ->
+          u >= length _tus ->
+          exists eUD : exprT (_tus' ++ tus') tvs (typD t),
+            exprD' (_tus' ++ tus') tvs
+                   (lookup_compress es (length _tus') (u - length _tus)) t =
+            Some eUD /\
+            (forall _us _us' us us' vs,
+                R _us _us' vs us us' ->
+                get (hlist_app _us us) = eUD (hlist_app _us' us') vs).
+    Proof.
+      clear base_is_nus. clear c cs base.
+      induction 1.
+      { simpl; intros.
+        generalize (@UVar_exprD' typ expr _ _ _ _ (_tus' ++ tus) _tvs (length _tus' + (u - length _tus)) t).
+        destruct (exprD' (_tus' ++ tus) _tvs (UVar (length _tus' + (u - length _tus))) t).
+        { intros; forward_reason.
+          eexists; split; eauto.
+          eapply nth_error_get_hlist_nth_appR in H; [ | omega ].
+          eapply nth_error_get_hlist_nth_appR in H2; [ | omega ].
+          simpl in *. forward_reason.
+          replace (length _tus' + (u - length _tus) - length _tus')
+             with (u - length _tus) in H2 by omega.
+          rewrite H in H2. inv_all; subst.
+          intros. subst.
+          specialize (H5 _us us').
+          specialize (H4 _us' us').
+          specialize (H3 (hlist_app _us' us') vs).
+          rewrite H5; clear H5.
+          rewrite <- H4; clear H4.
+          eassumption. }
+        { intro XXX; exfalso. clear - XXX H H1 H0.
+          eapply nth_error_get_hlist_nth_Some in H. simpl in H.
+          forward_reason.
+          clear H.
+          rewrite ListNth.nth_error_app_R in x by omega.
+          rewrite ListNth.nth_error_app_R in XXX by omega.
+          replace (length _tus' + (u - length _tus) - length _tus')
+             with (u - length _tus) in XXX by omega.
+          destruct XXX.
+          { congruence. }
+          { rewrite x in H.
+            forward_reason. eapply H2. inv_all. destruct H. apply Rrefl. } } }
+      { intros.
+        consider (u - length _tus).
+        { intros.
+          assert (u = length _tus) by omega.
+          subst. clear H3 H2.
+          simpl.
+          generalize (UVar_exprD' (_tus' ++ t :: tus') _tvs (length _tus') t0).
+          destruct (exprD' (_tus' ++ t :: tus') _tvs (UVar (length _tus')) t0).
+          { intros; forward_reason.
+            clear IHmapD.
+            eapply nth_error_get_hlist_nth_appR in H2; [ | omega ].
+            eapply nth_error_get_hlist_nth_appR in H0; [ | omega ].
+            simpl in *. rewrite Minus.minus_diag in *.
+            forward_reason; inv_all; subst.
+            eexists; split; eauto.
+            intros. destruct H0.
+            rewrite <- H3; clear H3.
+            rewrite H4; clear H4.
+            rewrite H5; clear H5.
+            subst.
+            revert H6. rewrite (UIP_refl x2).
+            intros; subst.
+            assumption. }
+          { clear IHmapD.
+            eapply nth_error_get_hlist_nth_Some in H0; forward_reason.
+            clear H0.
+            intro XXX; exfalso; clear - x XXX; simpl in *.
+            repeat rewrite ListNth.nth_error_app_R in * by omega.
+            rewrite Minus.minus_diag in *. simpl in *.
+            destruct XXX; forward_reason; try congruence. } }
+        { intros.
+          simpl.
+          specialize (IHmapD u).
+          repeat rewrite app_length in IHmapD. simpl in IHmapD.
+          replace (length _tus' + 1) with (S (length _tus')) in IHmapD by omega.
+          replace (u - (length _tus + 1)) with n in IHmapD by omega.
+          replace (length _tus + 1) with (S (length _tus)) in IHmapD by omega.
+          rewrite nth_error_get_hlist_nth_conv with (pf:=app_ass_trans _tus (t::nil) tus) in H0.
+          autorewrite with eq_rw in H0. forward.
+          destruct s. specialize (IHmapD _ _ eq_refl).
+          destruct IHmapD; [ omega | omega | forward_reason ].
+          inv_all; subst.
+          rewrite exprD'_conv with (pfu:=app_ass_trans _tus' (t::nil) tus') (pfv:=eq_refl).
+          revert H4. autorewrite with eq_rw. simpl.
+          intros. inv_all. subst.
+          rewrite H5. eexists; split; eauto.
+          intros.
+          subst.
+          destruct H4. eapply H6 in H7.
+          revert H7.
+          do 2 rewrite hlist_app_assoc.
+          autorewrite with eq_rw.
+          simpl.
+          rewrite (hlist_eta us).
+          rewrite (hlist_eta us'). simpl.
+          rewrite H4. auto. } }
+      { simpl; intros.
+        consider (u - length _tus).
+        { intros.
+          assert (u = length _tus) by omega.
+          subst. clear IHmapD H3 H4.
+          eapply nth_error_get_hlist_nth_appR in H1; [ | omega ].
+          simpl in H1. rewrite Minus.minus_diag in H1.
+          forward_reason; inv_all; subst. subst.
+          eexists; split; eauto.
+          intros; forward_reason.
+          rewrite H3; clear H3.
+          assumption. }
+        { intros.
+          rewrite nth_error_get_hlist_nth_conv with (pf:=app_ass_trans _tus (t::nil) tus) in H1.
+          autorewrite with eq_rw in H1.
+          specialize (IHmapD u).
+          forward.
+          autorewrite with eq_rw in H5.
+          inv_all; subst. subst.
+          destruct s; simpl in *.
+          destruct (IHmapD _ _ eq_refl); clear IHmapD.
+          { rewrite app_length; simpl; omega. }
+          { rewrite app_length; simpl; omega. }
+          forward_reason.
+          rewrite app_length in H5. simpl in *.
+          replace (u - (length _tus  + 1)) with n in H5 by omega.
+          eexists; split; eauto.
+          intros. forward_reason.
+          eapply H6 in H8.
+          rewrite <- H8; clear H8.
+          clear. autorewrite with eq_rw.
+          f_equal. rewrite hlist_app_assoc.
+          rewrite (hlist_eta us). simpl.
+          reflexivity. } }
+    Qed.
+
+    Axiom mapD_weaken_tvs : forall _tus _tus' _tvs _tvs' tus tus' es P,
+        @mapD _tus _tus' _tvs tus tus' es P ->
+        exists P',
+          @mapD _tus _tus' (_tvs ++ _tvs') tus tus' es P' /\
+          forall U U' V V' a b,
+            P U U' V a b <-> P' U U' (hlist_app V V') a b.
+
+    Hypothesis WF_cs : WellFormed_ctx_subst cs.
+
+    Lemma do_instantiate_sound
+      : forall (tus : list typ) (tvs : tenv typ) (tus' : list typ)
+               (R : hlist typD (getUVars c) -> hlist typD (getUVars c) ->
+                    hlist typD tvs -> hlist typD tus -> hlist typD tus' -> Prop)
+               (es : list (option expr)),
+        mapD tus tus' es R ->
+        forall sD,
+          ctx_substD (getUVars c) tvs cs = Some sD ->
+        forall (u : nat) (t : typ)
+               (get : hlist typD (getUVars c ++ tus) -> typD t),
+          nth_error_get_hlist_nth typD (getUVars c ++ tus) u =
+          Some
+            (existT (fun t0 : typ => hlist typD (getUVars c ++ tus) -> typD t0) t
+                    get) ->
+          match do_instantiate cs base es u with
+            | Some eU =>
+              exists eUD : exprT (getUVars c ++ tus') tvs (typD t),
+                exprD' (getUVars c ++ tus') tvs eU t = Some eUD /\
+                (forall (us : hlist typD (getUVars c ++ tus))
+                        (vs : hlist typD tvs) (us' : hlist typD (getUVars c ++ tus'))
+                        (vs' : hlist typD tvs),
+                    fst (hlist_split (getUVars c) tus us) =
+                    fst (hlist_split (getUVars c) tus' us') /\
+                    vs = vs' /\
+                    R (fst (hlist_split (getUVars c) tus us))
+                      (fst (hlist_split (getUVars c) tus us))
+                      vs
+                      (snd (hlist_split (getUVars c) tus us))
+                      (snd (hlist_split (getUVars c) tus' us')) ->
+                    sD (fst (hlist_split _ _ us)) vs ->
+                    get us = eUD us' vs')
+            | None =>
+              exists get' : hlist typD (getUVars c ++ tus') -> typD t,
+                nth_error_get_hlist_nth typD (getUVars c ++ tus') u =
+                Some
+                  (existT
+                     (fun t0 : typ => hlist typD (getUVars c ++ tus') -> typD t0) t
+                     get') /\
+                (forall (us : hlist typD (getUVars c ++ tus))
+                        (vs : hlist typD tvs) (us' : hlist typD (getUVars c ++ tus'))
+                        (vs' : hlist typD tvs),
+                    fst (hlist_split (getUVars c) tus us) =
+                    fst (hlist_split (getUVars c) tus' us') /\
+                    vs = vs' /\
+                    R (fst (hlist_split (getUVars c) tus us))
+                      (fst (hlist_split (getUVars c) tus us))
+                      vs
+                      (snd (hlist_split (getUVars c) tus us))
+                      (snd (hlist_split (getUVars c) tus' us')) /\
+                    sD (fst (hlist_split _ _ us)) vs ->
+                    get us = get' us')
+          end.
+    Proof.
+      unfold do_instantiate.
+      intros.
+      generalize (lt_rem_sound base u).
+      destruct (lt_rem u base); intros; forward_reason; subst.
+      { destruct (@lookup_compress_sound (getUVars c) (getUVars c) tus tus' tvs es _ H u _ _ H1).
+        { Instance Reflexive_ge : Reflexive ge.
+          Proof. constructor. Qed.
+          reflexivity. }
+        { assumption. }
+        { forward_reason.
+          eexists; split; eauto.
+          intros. forward_reason.
+          subst.
+          eapply H4 in H8.
+          repeat rewrite hlist_app_hlist_split in H8.
+          rewrite H5 in H8.
+          repeat rewrite hlist_app_hlist_split in H8.
+          assumption. } }
+      { consider (ctx_lookup u cs); intros.
+        { generalize (@substD_lookup (ctx_subst c) _ _ _ _ _ _ _ _ _
+                                     WF_cs H3 _ _ _ H0);
+          intros; forward_reason.
+          destruct (@nth_error_get_hlist_nth_appL _ typD tus _ _ H2).
+          rewrite H1 in H7. forward_reason; inv_all; subst; simpl in *.
+          eapply exprD'_weakenU with (tus':=tus') in H5; try eassumption.
+          destruct H5 as [ ? [ ? ? ] ].
+          rewrite H4 in H8. inv_all; subst.
+          eexists; split; eauto.
+          intros. forward_reason. subst.
+          specialize (H6 _ _ H10).
+          clear - H7 H9 H6 H8.
+          specialize (H7 (fst (hlist_split _ _ us)) vs'
+                         (snd (hlist_split _ _ us'))).
+          specialize (H9 (fst (hlist_split _ _ us)) (snd (hlist_split _ _ us))).
+          rewrite hlist_app_hlist_split in H9.
+          rewrite H8 in *.
+          rewrite hlist_app_hlist_split in H7.
+          etransitivity; eauto. etransitivity; eauto. }
+        { destruct (@nth_error_get_hlist_nth_appL _ typD tus _ _ H2).
+          destruct (@nth_error_get_hlist_nth_appL _ typD tus' _ _ H2).
+          forward_reason.
+          rewrite H8 in *. rewrite H5. rewrite H1 in *.
+          inv_all; subst. destruct x0; simpl in *.
+          subst. eexists; split; eauto.
+          intros. forward_reason. subst.
+          generalize (H9 (fst (hlist_split _ _ us))
+                         (snd (hlist_split _ _ us))); clear H9.
+          generalize (H7 (fst (hlist_split _ _ us'))
+                         (snd (hlist_split _ _ us'))); clear H7.
+          repeat rewrite hlist_app_hlist_split.
+          rewrite H4. clear.
+          intros. rewrite H0. symmetry; eassumption. } }
+    Qed.
+
+    Lemma instantiate_do_instantiate_sound
+    : forall (tus : list typ) (tvs : tenv typ) (tus' : list typ)
+             (e : expr)
+             (R : hlist typD (getUVars c) -> hlist typD (getUVars c) ->
+                  hlist typD tvs -> hlist typD tus -> hlist typD tus' -> Prop)
+             (es : list (option expr)),
+        mapD tus tus' es R ->
+        forall sD,
+          ctx_substD (getUVars c) tvs cs = Some sD ->
+        forall gD : exprT (getUVars c ++ tus) tvs Prop,
+          propD (getUVars c ++ tus) tvs e = Some gD ->
+          exists gD' : exprT (getUVars c ++ tus') tvs Prop,
+            propD (getUVars c ++ tus') tvs
+                  (instantiate (do_instantiate cs base es) 0 e) =
+            Some gD' /\
+            (forall (_us : hlist typD (getUVars c)) (_vs : hlist typD tvs)
+                    (us : hlist typD tus) (us' : hlist typD tus'),
+                R _us _us _vs us us' ->
+                sD _us _vs ->
+                (gD' (hlist_app _us us') _vs <-> gD (hlist_app _us us) _vs)).
+    Proof.
+      unfold propD, exprD'_typ0.
+      intros; forward; inv_all.
+      pose (R':=fun us vs us' vs' =>
+                 fst (hlist_split _ _ us) = fst (hlist_split _ _ us') /\
+                 vs = vs' /\
+                 R (fst (hlist_split _ _ us)) (fst (hlist_split _ _ us)) vs (snd (hlist_split _ _ us)) (snd (hlist_split _ _ us')) /\
+                 sD (fst (hlist_split _ _ us)) vs).
+      destruct (fun Hu Hv => @expr_subst_sound _ _ _ _ _
+                    (do_instantiate cs (length (getUVars c)) es) (fun _ => None) 0 e _ eq_refl
+                    nil (getUVars c ++ tus) tvs (getUVars c ++ tus') tvs
+                    R'
+                    Hu Hv
+                    (typ0 (F:=Prop)) _ eq_refl H1).
+      { (* Hu *)
+        intros.
+        generalize (@do_instantiate_sound _ _ _ _ _ H _ H0 _ _ _ H3).
+        subst.
+        destruct (do_instantiate cs (length (getUVars c)) es u).
+        { intros; forward_reason.
+          eexists; split; eauto.
+          subst R'. simpl. intros.
+          forward_reason.
+          eapply H4. eauto. eauto. }
+        { unfold R'. eauto. } }
+      { (* Hv *)
+        intros; eexists; split; eauto.
+        subst R'. simpl. intros. forward_reason.
+        subst. reflexivity. }
+      { forward_reason.
+        subst. change_rewrite H3.
+        eexists; split; eauto.
+        intros.
+        specialize (H4 (hlist_app _us us) _vs (hlist_app _us us') _vs Hnil).
+        subst R'. simpl in H4.
+        repeat rewrite hlist_split_hlist_app in H4. simpl in H4.
+        autorewrite with eq_rw. rewrite H4.
+        reflexivity. eauto. }
+    Qed.
+
+    (** TODO(gmalecha): move to bimap **)
+    Lemma only_in_range_empty : forall a b,
+        only_in_range a b (amap_empty expr).
+    Proof.
+      clear. red. intros.
+      eapply Forall_amap_empty.
+    Qed.
+
+    Lemma WellFormed_amap_amap_empty : WellFormed_amap (amap_empty expr).
+    Proof. red. eapply FMapSubst.SUBST.WellFormed_empty. Qed.
+
+    Lemma mapD_conv
+    : forall a b c us us' vs vs' es es' R
+             (pf_us:us=us') (pf_vs:vs=vs'),
+        es = es' ->
+        (@mapD a b c us vs es R <->
+         @mapD a b c us' vs' es'
+               match pf_us in _ = us
+                   , pf_vs in _ = vs
+                     return hlist _ a -> hlist _ b -> hlist _ c ->
+                            hlist _ us -> hlist _ vs -> Prop
+               with
+                 | eq_refl , eq_refl => R
+               end).
+    Proof.
+      clear. destruct pf_us. destruct pf_vs. intros; subst.
+      reflexivity.
+    Qed.
+
+    Fixpoint list_substD (tus tvs : tenv typ) (from : nat)
+             (es : list (option expr))
+      : option (exprT tus tvs Prop) :=
+      match es with
+        | nil => Some (fun _ _ => True)
+        | None :: es' =>
+          list_substD tus tvs (S from) es'
+        | Some e :: es' =>
+          match nth_error_get_hlist_nth _ tus from with
+            | None => None
+            | Some (existT t getU) =>
+              match exprD' tus tvs e t with
+                | None => None
+                | Some eD =>
+                  match list_substD tus tvs (S from) es' with
+                    | None => None
+                    | Some sD => Some (fun us vs =>
+                                         getU us = eD us vs /\ sD us vs)
+                  end
+              end
+          end
+      end.
+
+    (** What is missing here is the fact that [amap_substD a]
+     ** is equivalent to [list_substD tus tvs start ls]
+     **)
+    Theorem amap_substD_list_substD
+      : forall tus tvs am (from len : nat) sD maxV,
+        WellFormed_bimap from (from + len) maxV am ->
+        amap_substD tus tvs am = Some sD ->
+        exists sD',
+          list_substD tus tvs from (amap_aslist am from len) = Some sD' /\
+          forall us vs,
+            sD us vs <-> sD' us vs.
+    Proof. (** NOTE: this is not inductive **)
+    Admitted.
+
+    Lemma minify_goal_sound
+    : forall g tus tvs tus' es g',
+        minify_goal es (length (getUVars c ++ tus)) g = g' ->
+        WellFormed_Goal (getUVars c ++ tus) tvs g ->
+        WellFormed_Goal (getUVars c ++ tus') tvs g' /\
+        forall gD sD R,
+          goalD (getUVars c ++ tus) tvs g = Some gD ->
+          substD (getUVars c) tvs cs = Some sD ->
+          @mapD (getUVars c) (getUVars c) tvs tus tus' es R ->
+          exists gD',
+            goalD (getUVars c ++ tus') tvs g' = Some gD' /\
+            forall _us _vs us us',
+              R _us _us _vs us us' ->
+              sD _us _vs ->
+              (gD' (hlist_app _us us') _vs <->
+               gD (hlist_app _us us) _vs).
+    Proof.
+      induction g.
+      { (* All *)
+(*
+        simpl. intros. inv_all.
+        specialize (@IHg tus (tvs ++ t :: nil) tus' es _ _ eq_refl H0
+                         (@mapD_weaken_tvs _ _ (t :: nil) _ _ _ _ H1));
+          forward_reason.
+        destruct (@GAll_do_solved_respects _ _ _ _ _ (getUVars c ++ tus') tvs t
+                   _ _ (Reflexive_EqGoal _ _ (minify_goal es (length (getUVars c ++ tus)) g))). *)
+(*
+        split.
+        { subst. eapply H4.
+          constructor; assumption. }
+        intros; forward; inv_all; subst.
+        simpl.
+        specialize (H6 _ eq_refl).
+        forward_reason; Cases.rewrite_all_goal.
+        simpl in H5. rewrite H in H5.
+        inversion H5.
+        eexists; split; eauto.
+        simpl. intros. subst.
+        etransitivity. eapply H9. reflexivity. reflexivity.
+        eapply forall_iff. intro.
+        specialize (H6 _us (hlist_app _vs (Hcons x1 Hnil)) us us').
+        rewrite hlist_split_hlist_app in H6. simpl in H6. eauto. *) admit. }
+      { (* Exs *)
+        cbv beta iota delta [ minify_goal ]; fold minify_goal.
+        intros.
+        simpl in H.
+        remember (amap_aslist a (length (getUVars c ++ tus)) (length l)) as mlist.
+        remember (combine l
+                   (map
+                      (fun x : option expr =>
+                       match x with
+                       | Some x0 =>
+                           Some
+                             (instantiate (do_instantiate cs base (es ++ mlist))
+                                0 x0)
+                       | None => None
+                       end) mlist)) as tes.
+        remember (map fst
+                    (filter
+                       (fun x : typ * option expr =>
+                          match snd x with
+                            | Some _ => false
+                            | None => true
+                          end) tes)) as ts'.
+        remember (map
+                    (fun x : option expr =>
+                       match x with
+                         | Some x0 =>
+                           Some
+                             (instantiate (do_instantiate cs base (es ++ mlist)) 0
+                                          x0)
+                         | None => None
+                       end) mlist) as mlist_inst.
+        rename l into ts.
+        inv_all.
+        rewrite app_ass in H1.
+        specialize (IHg (tus ++ ts) tvs (tus' ++ ts') (es ++ mlist_inst) _
+                        eq_refl H1).
+        forward_reason.
+        destruct (@GExs_nil_check_respects _ _ _ _ _ _
+                    (getUVars c ++ tus') tvs ts' (amap_empty expr)
+                    (only_in_range_empty _ _)
+                    (WellFormed_amap_amap_empty) _ _
+                    (Reflexive_EqGoal _ _
+                       (minify_goal (es ++ mlist_inst)
+                          (length ts + length (getUVars c ++ tus)) g))).
+        split.
+        { subst g'.
+          eapply H4.
+          constructor.
+          eapply WellFormed_bimap_empty; eauto.
+          revert H0. clear.
+          repeat rewrite app_length.
+          rewrite app_ass.
+          match goal with
+            | |- ?X -> ?Y => cutrewrite (X = Y); try auto
+          end.
+          f_equal. f_equal. omega. }
+        clear H4.
+        rewrite H in *. clear H. (* Can I do this? *)
+        simpl in *; intros. forward; inv_all. subst gD.
+        rewrite goalD_conv with (pfu:=eq_sym (app_ass_trans _ _ _)) (pfv:=eq_refl) in H.
+        autorewrite with eq_rw in H. forward.
+        pose (R':=fun U U' V (a : hlist typD (tus ++ ts))
+                        (b : hlist typD (tus' ++ ts')) =>
+                      R U U' V (fst (hlist_split _ _ a)) (fst (hlist_split _ _ b))
+                      /\ e0 (hlist_app (hlist_app U (fst (hlist_split _ _ a)))
+                                       (snd (hlist_split _ _ a)))  V).
+        assert (exists R'',
+                   mapD (tus ++ ts) (tus' ++ ts') (es ++ mlist_inst) R'' /\
+                   forall _us _us' _vs a b,
+                     R'' _us _us' _vs a b <-> R' _us _us' _vs a b).
+        { clear H3 H H5. revert H6.
+          revert H7. subst mlist_inst.
+          revert Heqmlist. revert H2. subst R'.
+          revert Heqts'. subst tes.
+          clear. revert e0. revert R.
+          revert mlist ts' es. revert tus tvs tus'. revert a.
+          induction ts.
+          { simpl. intros; subst. simpl in *.
+            clear - H6 H7.
+            eapply mapD_conv
+              with (pf_us:=eq_sym (app_nil_r_trans _))
+                   (pf_vs:=eq_sym (app_nil_r_trans _))
+                   (es':=es++nil)
+              in H6; [ | symmetry; eapply app_nil_r_trans ].
+            eexists; split; eauto.
+            intros.
+            autorewrite with eq_rw.
+            rewrite (hlist_eta (snd (hlist_split _ _ a0))).
+            rewrite hlist_app_nil_r.
+            admit. }
+          { admit. } }
+(*
+        specialize (H3 _ _ R' eq_refl H4 H9).
+        forward_reason.
+        revert H5.
+        rewrite goalD_conv with (pfu:=eq_sym (app_ass_trans _ _ _)) (pfv:=eq_refl). autorewrite with eq_rw.
+        revert H3. repeat rewrite app_length.
+        replace (length (getUVars c) + (length tus + length ts))
+           with (length ts + (length (getUVars c) + length tus)) by omega.
+        intro XXX; rewrite XXX.
+        inversion 1. eexists; split; eauto.
+        intros. do 5 red in H12.
+        etransitivity; [ symmetry; eapply H12; reflexivity | ].
+*)
+        (** TODO(gmalecha): this should work out **)
+        admit. (* hard *) }
+      { (* Hyp *)
+        simpl. intros.
+        inv_all.
+        specialize (IHg tus tvs tus' es _ eq_refl H0).
+        forward_reason.
+        split.
+        { subst. eapply WellFormed_Goal_GHyp_do_solved.
+          constructor. eauto. }
+        { intros.
+          forwardy. inv_all; subst.
+          eapply instantiate_do_instantiate_sound in H3; eauto.
+          forward_reason.
+          generalize (@GHyp_do_solved_respects typ expr _ _ _ _ _ _ _ H).
+          unfold EqGoal; simpl. intros.
+          red in H7.
+          destruct (H7 (minify_goal es (length (getUVars c ++ tus)) g) (minify_goal es (length (getUVars c ++ tus)) g)); clear H7.
+          { clear. split; eauto. reflexivity.
+            apply Option.Reflexive_Roption.
+            eapply Reflexive_RexprT. eauto with typeclass_instances. }
+          revert H9; simpl.
+          eapply H2 in H6; clear H2; eauto.
+          forward_reason.
+          Cases.rewrite_all_goal.
+          intros. inversion H9; clear H9; subst.
+          eexists; split; eauto.
+          intros.
+          specialize (H6 _ _ _ _ H9 H10).
+          specialize (H3 _ _ _ _ H9 H10).
+          rewrite <- H6; clear H6.
+          rewrite <- H3; clear H3.
+          eapply H11. reflexivity. reflexivity. } }
+      { (* Conj *)
+        admit. (* medium *) }
+      { (* Goal *)
+        intros. clear base_is_nus. subst.
+        split.
+        { constructor. }
+        simpl in *. intros.
+        eapply instantiate_do_instantiate_sound; eauto. }
+      { (* Solved *)
+        intros; clear base_is_nus; subst.
+        split; [ constructor | ].
+        intros; inv_all; subst.
+        simpl. eexists; split; eauto.
+        simpl. reflexivity. }
+    Qed.
 
   End minify.
 
@@ -132,7 +787,49 @@ Section parameterized.
     eapply Proper_rtacK_spec;
       [ reflexivity | eapply More_More_; reflexivity | ].
     red.
-    intros; split; auto.
-  Admitted.
+    intros.
+    rewrite <- (app_nil_r_trans (getUVars ctx)) in H.
+    destruct (@minify_goal_sound _ _ s eq_refl H0 g nil
+                                 (getVars ctx) nil nil _ eq_refl H).
+    split; auto.
+    split.
+    { clear - H1. rewrite app_nil_r_trans in H1. assumption. }
+    forward.
+    rewrite goalD_conv with (pfu:=app_nil_r_trans _) (pfv:=eq_refl) in H4.
+    autorewrite with eq_rw in H4.
+    forward.
+    destruct (@pctxD_substD  _ _ _ _ _ _ _ _ _ _ H0 H3); forward_reason.
+    specialize (H4 _ _ _ eq_refl H6 (@MD_nil _ _ _ _)).
+    forward_reason.
+    inv_all; subst.
+    rewrite goalD_conv with (pfu:=app_nil_r_trans _) (pfv:=eq_refl).
+    autorewrite with eq_rw.
+    cutrewrite (minify_goal (length (getUVars ctx)) s nil (length (getUVars ctx)) g = minify_goal (length (getUVars ctx)) s nil (length (getUVars ctx ++ nil)) g).
+    { rewrite H4.
+      split; [ reflexivity | ].
+      intros. gather_facts.
+      eapply Pure_pctxD; eauto. clear - H8.
+      intros. specialize (H8 us vs Hnil Hnil eq_refl H).
+      revert H0. autorewrite with eq_rw.
+      rewrite <- hlist_app_nil_r. eapply H8. }
+    { f_equal. rewrite app_nil_r_trans. reflexivity. }
+  Qed.
 
 End parameterized.
+
+(*
+Lemma minify_goal_sound
+    : forall g tus tvs tus' es g' R,
+        (minify_goal es (length (getUVars c ++ tus)) g) = g' ->
+        WellFormed_Goal (getUVars c ++ tus) (getVars c ++ tvs) g ->
+        @mapD (getUVars c) (getVars c ++ tvs) tus tus' es R ->
+        WellFormed_Goal (getUVars c ++ tus') (getVars c ++ tvs) g' /\
+        forall gD,
+          goalD (getUVars c ++ tus) (getVars c ++ tvs) g = Some gD ->
+          exists gD',
+            goalD (getUVars c ++ tus') (getVars c ++ tvs) g' = Some gD' /\
+            forall _us _vs us us' vs,
+              R _us (hlist_app _vs vs) us us' ->
+              (gD' (hlist_app _us us') (hlist_app _vs vs) <->
+               gD (hlist_app _us us) (hlist_app _vs vs)).
+*)
